proof: soundness of AttrClosureImpl

RelationalAlgebra/NF/Closure.lean
@@ -2,7 +2,10 @@ import RelationalAlgebra.NF.FuncDep
 import RelationalAlgebra.NF.Misc
 
 import Mathlib.Data.Finset.Basic
+import Mathlib.Data.Finset.Defs
+import Mathlib.Data.Finset.Insert
 import Mathlib.Data.Finset.Lattice.Basic
+import Mathlib.Data.Finset.Lattice.Fold
 
 namespace RM
 
@@ -38,7 +41,7 @@ inductive Derives (F : Finset (FunctionalDependency α)) : FunctionalDependency 
 infix:50 " ⊢ " => Derives
 
 /-- Soundness of Armstrong's Axioms: if F ⊢ f, then F ⊨ f. -/
-theorem armstrong_soundness {F : Finset (FunctionalDependency α)} {f : FunctionalDependency α} :
+theorem armstrong_sound {F : Finset (FunctionalDependency α)} {f : FunctionalDependency α} :
   F ⊢ f → F ⊨ f := by
   intro h_der μ r h_sat
   induction h_der with
@@ -66,7 +69,7 @@ theorem armstrong_soundness {F : Finset (FunctionalDependency α)} {f : Function
       exact h_xy_holds t₁ t₂ h_t₁ h_t₂ h_eq_x a h_a_in_y
     exact h_yz_holds t₁ t₂ h_t₁ h_t₂ h_eq_y s h_s_in_z
 
-theorem armstrong_completeness {F : Finset (FunctionalDependency α)} {f : FunctionalDependency α} :
+theorem armstrong_complete {F : Finset (FunctionalDependency α)} {f : FunctionalDependency α} :
   F ⊨ f → F ⊢ f := by
   sorry
 
@@ -86,14 +89,10 @@ theorem derives_decomposition {F : Finset (FunctionalDependency α)} {X Y Z : Fi
   F ⊢ (X -> Y ∪ Z) → F ⊢ (X -> Y) ∧ F ⊢ (X -> Z) := by
   intro h_der_x_yz
   constructor
-  {
-    have h_der_yz_y : F ⊢ (Y ∪ Z -> Y) := by simpa using Derives.reflexivity (Y ∪ Z) Y
+  · have h_der_yz_y : F ⊢ (Y ∪ Z -> Y) := by simpa using Derives.reflexivity (Y ∪ Z) Y
     exact Derives.transitivity X (Y ∪ Z) Y h_der_x_yz h_der_yz_y
-  }
-  {
-    have h_der_yz_z : F ⊢ (Y ∪ Z -> Z) := by simpa using Derives.reflexivity (Y ∪ Z) Z
+  · have h_der_yz_z : F ⊢ (Y ∪ Z -> Z) := by simpa using Derives.reflexivity (Y ∪ Z) Z
     exact Derives.transitivity X (Y ∪ Z) Z h_der_x_yz h_der_yz_z
-  }
 
 /-- b₃ (Pseudotransitivity): if X -> Y and YZ -> W, then XZ -> W. -/
 theorem derives_pseudotransitivity {F : Finset (FunctionalDependency α)} {X Y Z W : Finset α} :
@@ -107,8 +106,8 @@ end Armstrong
 section FuncDepClosure
 
 /-- F⁺: Closure of a FD set. -/
-def FuncDepClosure (F : Finset (FunctionalDependency α)) : Finset (FunctionalDependency α) :=
-  sorry
+def FuncDepClosure (F : Finset (FunctionalDependency α)) : Set (FunctionalDependency α) :=
+  {f | F ⊨ f}
 
 /--
   F⁺ contains **all** FDs implied by F.
@@ -123,7 +122,65 @@ end FuncDepClosure
 section AttrClosure
 
 /-- X⁺: Closure of an attribute set X with respect to a FD set, F. -/
-def AttrClosure (F : Finset (FunctionalDependency α)) (X : Finset α) : Finset α :=
+def AttrClosure (F : Finset (FunctionalDependency α)) (X : Finset α) : Set α :=
+  {a | (X -> {a} : FunctionalDependency α) ∈ FuncDepClosure F}
+
+/--
+  Single step iteration for computing the attribute set closure.
+  If α -> β is in F and α ⊆ X, then we can add β to X.
+-/
+def _attrClosureStep (F : Finset (FunctionalDependency α)) (X : Finset α) : Finset α :=
+  have f_filtered := {fd ∈ F | fd.lhs ⊆ X}
+  X ∪ f_filtered.sup (λ fd => fd.rhs)
+
+/-- Implementation of attribute set closure, where we iterate the single step |F| times (in the worst case). -/
+def AttrClosureImpl (F : Finset (FunctionalDependency α)) (X : Finset α) : Finset α :=
+  (_attrClosureStep F)^[F.card] X
+
+lemma attr_closure_step_sound {F : Finset (FunctionalDependency α)} {X : Finset α} :
+  F ⊢ (X -> _attrClosureStep F X) := by
+  simp [_attrClosureStep]
+  apply derives_union
+  · apply Derives.reflexivity
+    simp
+  · set s := {fd ∈ F | fd.lhs ⊆ X}
+    have h_s_subset_F : s ⊆ F := by simp [s]
+    have h_s'_sup : ∀ s' ⊆ s, F ⊢ (X -> s'.sup (λ fd => fd.rhs)) := by
+      intro s' h_s'_sub_s
+      induction s' using Finset.induction with
+      | empty => simp [Derives.reflexivity]
+      | insert fd s'' h_fd_not_in_s'' h_ih =>
+        simp [Finset.sup_insert]
+        obtain ⟨h_fd, h_s''⟩ := Finset.insert_subset_iff.mp h_s'_sub_s
+        apply derives_union
+        · apply Derives.transitivity X fd.lhs fd.rhs
+          · apply Derives.reflexivity
+            simp [Finset.mem_filter.mp h_fd]
+          · apply Derives.member
+            have h_fd_in_F : fd ∈ F := by apply Finset.mem_of_subset h_s_subset_F h_fd
+            exact h_fd_in_F
+        · exact h_ih h_s''
+    apply h_s'_sup s
+    simp
+
+lemma attr_closure_iterate_sound {F : Finset (FunctionalDependency α)} {X : Finset α} (n : ℕ) :
+  F ⊢ (X -> (_attrClosureStep F)^[n] X) := by
+  induction n with
+  | zero => simp [Derives.reflexivity]
+  | succ n ih =>
+    apply Derives.transitivity X ((_attrClosureStep F)^[n] X) ((_attrClosureStep F)^[n + 1] X)
+    · exact ih
+    · rw [Function.iterate_succ_apply']
+      set Y := (_attrClosureStep F)^[n] X
+      exact attr_closure_step_sound
+
+lemma attr_closure_sound {F : Finset (FunctionalDependency α)} {X : Finset α} :
+  F ⊢ (X -> AttrClosureImpl F X) := by
+  simp [AttrClosureImpl]
+  exact attr_closure_iterate_sound F.card
+
+lemma attr_closure_complete {F : Finset (FunctionalDependency α)} {X : Finset α} (a : α) :
+  F ⊢ (X -> Y) → Y ⊆ AttrClosureImpl F X := by
   sorry
 
 /--
@@ -131,22 +188,7 @@ def AttrClosure (F : Finset (FunctionalDependency α)) (X : Finset α) : Finset 
   Correctness = Validity (X -> X⁺ ∈ F⁺) + Maximality (∀ β, X -> β ∈ F⁺ → β ⊆ X⁺)
 -/
 theorem attr_closure_correct {F : Finset (FunctionalDependency α)} {X : Finset α} :
-  ((X -> AttrClosure F X) : FunctionalDependency α) ∈ FuncDepClosure F
-  ∧ ∀ β : Finset α, ((X -> β) : FunctionalDependency α) ∈ FuncDepClosure F → β ⊆ AttrClosure F X := by
-  sorry
-
--- The above proof requires the computation of F⁺, which is exponential.
--- Since we only check the membership of an FD in F⁺, we have:
--- f ∈ F⁺ ↔ F ⊨ f
-
-theorem attr_closure_correct_alt {F : Finset (FunctionalDependency α)} {X : Finset α} :
-  F ⊨ (X -> AttrClosure F X) ∧ ∀ β : Finset α, F ⊨ (X -> β) → β ⊆ AttrClosure F X := by
-  sorry
-
--- And, since we have the soundness of Armstrong's axioms, we can use derivation instead of implication, which is more computationally tractable.
-
-theorem attr_closure_correct_alt2 {F : Finset (FunctionalDependency α)} {X : Finset α} :
-  F ⊢ (X -> AttrClosure F X) ∧ ∀ β : Finset α, F ⊢ (X -> β) → β ⊆ AttrClosure F X := by
+  AttrClosureImpl F X = AttrClosure F X := by
   sorry
 
 /-- Syntactic superkey: a set of attributes K is a superkey with respect to a set of functional dependencies F if F implies K -> r.schema. -/
@@ -174,7 +216,7 @@ theorem structSuperkeyImpliesSemanticSuperkey {r : RelationInstance α μ} {F : 
   We simplify the left-hand side using f ∈ F⁺ ↔ F ⊨ f.
 -/
 theorem funcDepValidityViaAttrClosure {r : RelationInstance α μ} {F : Finset (FunctionalDependency α)} {S T : Finset α} :
-  S ⊆ r.schema → T ⊆ r.schema → F ⊨ (S -> T) ↔ T ⊆ AttrClosure F S := by
+  S ⊆ r.schema → T ⊆ r.schema → F ⊨ (S -> T) ↔ T ⊆ AttrClosureImpl F S := by
   sorry
 
 end AttrClosure
